spec/abstract/RISCV64/ArchTcb_A.thy
@@ -8,10 +8,6 @@
  * @TAG(DATA61_GPL)
  *)
 
-(*
-Arch-specific functions for the abstract model of CSpace.
-*)
-
 chapter "Architecture-specific TCB functions"
 
 theory ArchTcb_A
@@ -20,27 +16,22 @@ begin
 
 context Arch begin global_naming RISCV64_A
 
-definition
-  arch_tcb_set_ipc_buffer :: "machine_word \<Rightarrow> vspace_ref \<Rightarrow> (unit, 'a::state_ext) s_monad"
-where
+definition arch_tcb_set_ipc_buffer :: "machine_word \<Rightarrow> vspace_ref \<Rightarrow> (unit, 'a::state_ext) s_monad"
+  where
   "arch_tcb_set_ipc_buffer target ptr \<equiv> as_user target $ setRegister TP ptr"
 
-(* Allow most pre-existing proofs to continue to work. *)
 declare arch_tcb_set_ipc_buffer_def [simp]
 
-definition
-  sanitise_register :: "bool \<Rightarrow> register \<Rightarrow> machine_word \<Rightarrow> machine_word"
-where
+definition sanitise_register :: "bool \<Rightarrow> register \<Rightarrow> machine_word \<Rightarrow> machine_word"
+  where
   "sanitise_register t r v \<equiv> v"
 
-definition
-  arch_get_sanitise_register_info :: "obj_ref \<Rightarrow> (bool, 'a::state_ext) s_monad"
-where
+definition arch_get_sanitise_register_info :: "obj_ref \<Rightarrow> (bool, 'a::state_ext) s_monad"
+  where
   "arch_get_sanitise_register_info t \<equiv> return False"
 
-definition
-  arch_post_modify_registers :: "obj_ref \<Rightarrow> obj_ref \<Rightarrow> (unit, 'a::state_ext) s_monad"
-where
+definition arch_post_modify_registers :: "obj_ref \<Rightarrow> obj_ref \<Rightarrow> (unit, 'a::state_ext) s_monad"
+  where
   "arch_post_modify_registers cur t \<equiv> return ()"
 
 end
