spec/abstract/RISCV64/Hypervisor_A.thy
@@ -8,7 +8,7 @@
  * @TAG(DATA61_GPL)
  *)
 
-chapter "Handle Hyperviser Fault Event"
+chapter "Handle Hypervisor Fault Events"
 
 theory Hypervisor_A
 imports "../Exceptions_A"
@@ -17,8 +17,8 @@ begin
 context Arch begin global_naming RISCV64_A
 
 fun handle_hypervisor_fault :: "machine_word \<Rightarrow> hyp_fault_type \<Rightarrow> (unit, 'z::state_ext) s_monad"
-where
-"handle_hypervisor_fault thread RISCVNoHypFaults = return ()"
+  where
+  "handle_hypervisor_fault thread RISCVNoHypFaults = return ()"
 
 end
 end
